BVL-->BVP compiler transformed into BVI-->BVP compiler

new-backend/bvi_to_bvpScript.sml
@@ -1,18 +1,18 @@
-open HolKernel Parse boolLib bossLib; val _ = new_theory "bvl_to_bvp";
+open HolKernel Parse boolLib bossLib; val _ = new_theory "bvi_to_bvp";
 
 open pred_setTheory arithmeticTheory pairTheory listTheory combinTheory;
 open finite_mapTheory sumTheory relationTheory stringTheory optionTheory;
 open bytecodeTheory bvlTheory bvl_constTheory;
 open bvl_inlineTheory bvpTheory;
 open bvp_lemmasTheory bvp_simpTheory bvp_liveTheory bvp_spaceTheory;
-open sptreeTheory lcsymtacs;
+open sptreeTheory lcsymtacs bviTheory;
 
 infix \\ val op \\ = op THEN;
 
-(* compilation from BVL to BVP *)
+(* compilation from BVI to BVP *)
 
-val bAssign_def = Define `
-  bAssign n1 op vs live env =
+val iAssign_def = Define `
+  iAssign n1 op vs live env =
     if op_space_reset op then
       Assign n1 op vs (SOME (list_to_num_set (vs++live++env)))
     else
@@ -21,55 +21,54 @@ val bAssign_def = Define `
           else Seq (MakeSpace k (list_to_num_set (vs++live++env)))
                    (Assign n1 op vs NONE)`;
 
-val bComp_def = tDefine "bComp" `
-  (bComp (n:num) (env:num list) tail live [] =
+val iComp_def = tDefine "iComp" `
+  (iComp (n:num) (env:num list) tail live [] =
     (Skip,[]:num list,n)) /\
-  (bComp n env tail live (x::y::xs) =
-     let (c1,v1,n1) = bComp n env F live [x] in
-     let (c2,vs,n2) = bComp n1 env F (HD v1::live) (y::xs) in
+  (iComp n env tail live (x::y::xs) =
+     let (c1,v1,n1) = iComp n env F live [x] in
+     let (c2,vs,n2) = iComp n1 env F (HD v1::live) (y::xs) in
        (Seq c1 c2, HD v1 :: vs, n2)) /\
-  (bComp n env tail live [Var v] =
+  (iComp n env tail live [(Var v):bvi_exp] =
      if tail
      then (Return (EL v env), [n], n+1)
      else (Move n (EL v env), [n], n+1)) /\
-  (bComp n env tail live [If x1 x2 x3] =
-     let (c1,v1,n1) = bComp n env F live [x1] in
-     let (c2,v2,n2) = bComp n1 env tail live [x2] in
-     let (c3,v3,n3) = bComp n2 env tail live [x3] in
+  (iComp n env tail live [If x1 x2 x3] =
+     let (c1,v1,n1) = iComp n env F live [x1] in
+     let (c2,v2,n2) = iComp n1 env tail live [x2] in
+     let (c3,v3,n3) = iComp n2 env tail live [x3] in
        if tail then
          (If c1 (HD v1) c2 c3,[n3],n3+1)
        else
          (If c1 (HD v1) (Seq c2 (Move n3 (HD v2)))
                         (Seq c3 (Move n3 (HD v3))),[n3],n3+1)) /\
-  (bComp n env tail live [Let xs x2] =
-     let (c1,vs,n1) = bComp n env F live xs in
-     let (c2,v2,n2) = bComp n1 (vs ++ env) tail live [x2] in
+  (iComp n env tail live [Let xs x2] =
+     let (c1,vs,n1) = iComp n env F live xs in
+     let (c2,v2,n2) = iComp n1 (vs ++ env) tail live [x2] in
        (Seq c1 c2, v2, n2)) /\
-  (bComp n env tail live [Raise x1] =
-     let (c1,v1,n1) = bComp n env F live [x1] in
+  (iComp n env tail live [Raise x1] =
+     let (c1,v1,n1) = iComp n env F live [x1] in
        (Seq c1 (Raise (HD v1)), v1, n1)) /\
-  (bComp n env tail live [Handle x1 x2] = (Skip, [n], n)) /\
-  (bComp n env tail live [Op op xs] =
-     let (c1,vs,n1) = bComp n env F live xs in
-     let c2 = Seq c1 (bAssign n1 op vs live env) in
+  (iComp n env tail live [Op op xs] =
+     let (c1,vs,n1) = iComp n env F live xs in
+     let c2 = Seq c1 (iAssign n1 op vs live env) in
        (if tail then Seq c2 (Return n1) else c2, [n1], n1+1)) /\
-  (bComp n env tail live [Tick x1] =
-     let (c1,v1,n1) = bComp n env tail live [x1] in
+  (iComp n env tail live [Tick x1] =
+     let (c1,v1,n1) = iComp n env tail live [x1] in
        (Seq Tick c1, v1, n1)) /\
-  (bComp n env tail live [Call dest xs] =
-     let (c1,vs,n1) = bComp n env F live xs in
+  (iComp n env tail live [Call dest xs handler] =
+     let (c1,vs,n1) = iComp n env F live xs in
      let ret = (if tail then NONE
                 else SOME (n1, list_to_num_set (live ++ env))) in
        (Seq c1 (Call ret dest vs NONE), [n1], n1+1))`
- (WF_REL_TAC `measure (bvl_exp1_size o SND o SND o SND o SND)`);
+ (WF_REL_TAC `measure (bvi_exp2_size o SND o SND o SND o SND)`);
 
 val pOptimise_def = Define `
   pOptimise prog = pSpaceOpt (FST (pLive (pSimp prog Skip) LN))`;
 
-val bCompile_def = Define `
-  bCompile arg_count exp =
+val iCompile_def = Define `
+  iCompile arg_count exp =
     let env = GENLIST I arg_count in
-      pOptimise (FST (bComp arg_count env T [] [exp]))`;
+      pOptimise (FST (iComp arg_count env T [] [exp]))`;
 
 (* verification proof *)
 
@@ -90,41 +89,41 @@ val var_corr_def = Define `
   var_corr env corr t <=>
     EVERY2 (\v x. get_var v t = SOME x) corr env`;
 
-val bComp_LESS_EQ_lemma = prove(
+val iComp_LESS_EQ_lemma = prove(
   ``!n env tail live xs.
-      n <= SND (SND (bComp n env tail live xs))``,
-  HO_MATCH_MP_TAC (fetch "-" "bComp_ind") \\ REPEAT STRIP_TAC
-  \\ SIMP_TAC std_ss [bComp_def] \\ SRW_TAC [] []
+      n <= SND (SND (iComp n env tail live xs))``,
+  HO_MATCH_MP_TAC (fetch "-" "iComp_ind") \\ REPEAT STRIP_TAC
+  \\ SIMP_TAC std_ss [iComp_def] \\ SRW_TAC [] []
   \\ FULL_SIMP_TAC (srw_ss()) [] \\ SRW_TAC [] [] \\ DECIDE_TAC);
 
-val bComp_LESS_EQ = store_thm("bComp_LESS_EQ",
+val iComp_LESS_EQ = store_thm("iComp_LESS_EQ",
   ``!n env tail live xs c vs new_var.
-      (bComp n env tail live xs = (c,vs,new_var)) ==> n <= new_var``,
-  REPEAT STRIP_TAC \\ MP_TAC (SPEC_ALL bComp_LESS_EQ_lemma)
+      (iComp n env tail live xs = (c,vs,new_var)) ==> n <= new_var``,
+  REPEAT STRIP_TAC \\ MP_TAC (SPEC_ALL iComp_LESS_EQ_lemma)
   \\ FULL_SIMP_TAC std_ss []);
 
-val bComp_LENGTH_lemma = prove(
+val iComp_LENGTH_lemma = prove(
   ``!n env tail live xs.
-      (LENGTH (FST (SND (bComp n env tail live xs))) = LENGTH xs)``,
-  HO_MATCH_MP_TAC (fetch "-" "bComp_ind") \\ REPEAT STRIP_TAC
-  \\ SIMP_TAC std_ss [bComp_def] \\ SRW_TAC [] []
+      (LENGTH (FST (SND (iComp n env tail live xs))) = LENGTH xs)``,
+  HO_MATCH_MP_TAC (fetch "-" "iComp_ind") \\ REPEAT STRIP_TAC
+  \\ SIMP_TAC std_ss [iComp_def] \\ SRW_TAC [] []
   \\ FULL_SIMP_TAC (srw_ss()) [] \\ SRW_TAC [] []);
 
-val bComp_LENGTH = store_thm("bComp_LENGTH",
+val iComp_LENGTH = store_thm("iComp_LENGTH",
   ``!n env tail live xs c vs new_var.
-      (bComp n env tail live xs = (c,vs,new_var)) ==> (LENGTH vs = LENGTH xs)``,
-  REPEAT STRIP_TAC \\ MP_TAC (SPEC_ALL bComp_LENGTH_lemma)
+      (iComp n env tail live xs = (c,vs,new_var)) ==> (LENGTH vs = LENGTH xs)``,
+  REPEAT STRIP_TAC \\ MP_TAC (SPEC_ALL iComp_LENGTH_lemma)
   \\ FULL_SIMP_TAC std_ss []);
 
-val bComp_SING_IMP = prove(
-  ``(bComp n env tail live [x] = (c,vs,new_var)) ==> ?t. vs = [t]``,
-  REPEAT STRIP_TAC \\ IMP_RES_TAC bComp_LENGTH
+val iComp_SING_IMP = prove(
+  ``(iComp n env tail live [x] = (c,vs,new_var)) ==> ?t. vs = [t]``,
+  REPEAT STRIP_TAC \\ IMP_RES_TAC iComp_LENGTH
   \\ Cases_on `vs` \\ FULL_SIMP_TAC (srw_ss()) []
   \\ Cases_on `t` \\ FULL_SIMP_TAC (srw_ss()) []);
 
-val bEval_SING_IMP = prove(
-  ``(bEval ([x],env,s1) = (Result vs,s2)) ==> ?w. vs = [w]``,
-  REPEAT STRIP_TAC \\ IMP_RES_TAC bEval_length
+val iEval_SING_IMP = prove(
+  ``(iEval ([x],env,s1) = (Result vs,s2)) ==> ?w. vs = [w]``,
+  REPEAT STRIP_TAC \\ IMP_RES_TAC iEval_IMP_LENGTH
   \\ Cases_on `vs` \\ FULL_SIMP_TAC (srw_ss()) []
   \\ Cases_on `t` \\ FULL_SIMP_TAC (srw_ss()) []);
 
@@ -158,14 +157,15 @@ val LIST_REL_REVERSE = prove(
   \\ REPEAT STRIP_TAC \\ FULL_SIMP_TAC std_ss [LIST_REL_SNOC] \\ METIS_TAC []);
 
 val code_rel_def = Define `
-  code_rel bvl_code bvp_code <=>
-    (domain bvl_code = domain bvp_code) /\
+  code_rel bvi_code bvp_code <=>
+    wf bvi_code /\ wf bvp_code /\
+    (domain bvi_code = domain bvp_code) /\
     !n exp arg_count.
-      (lookup n bvl_code = SOME (arg_count,exp)) ==>
-      (lookup n bvp_code = SOME (arg_count,bCompile arg_count exp))`;
+      (lookup n bvi_code = SOME (arg_count,exp)) ==>
+      (lookup n bvp_code = SOME (arg_count,iCompile arg_count exp))`;
 
 val state_rel_def = Define `
-  state_rel (s:bvl_state) (t:bvp_state) <=>
+  state_rel (s:bvi_state) (t:bvp_state) <=>
     (s.clock = t.clock) /\
     code_rel s.code t.code /\
     (s.globals = t.globals) /\
@@ -181,7 +181,7 @@ val get_vars_thm = prove(
 val find_code_lemma = prove(
   ``state_rel r t2 /\
     (find_code dest a r.code = SOME (args,exp)) ==>
-    (find_code dest a t2.code = SOME (args,bCompile (LENGTH args) exp))``,
+    (find_code dest a t2.code = SOME (args,iCompile (LENGTH args) exp))``,
   REVERSE (Cases_on `dest`) \\ SIMP_TAC std_ss [find_code_def]
   \\ FULL_SIMP_TAC (srw_ss()) [state_rel_def,code_rel_def]
   \\ REPEAT STRIP_TAC THEN1
@@ -255,27 +255,106 @@ val s_space_ID = prove(
 
 val get_vars_add_space = prove(
   ``!vs s x. (get_vars vs (add_space s x) = get_vars vs s) /\
-             (get_vars vs (add_space s x with locals := y) = get_vars vs (s with locals := y))``,
+             (get_vars vs (add_space s x with locals := y) =
+              get_vars vs (s with locals := y))``,
   Induct \\ fs [get_vars_def,get_var_def,add_space_def]);
 
-val bEvalOp_code = prove(
-  ``!op s1 s2. (bEvalOp op a s1 = SOME (x0,s2)) ==> (s2.code = s1.code)``,
-  METIS_TAC [bEvalOp_const]);
+val iEvalOp_code = prove(
+  ``!op s1 s2. (iEvalOp op a s1 = SOME (x0,s2)) ==> (s2.code = s1.code)``,
+  SIMP_TAC std_ss [iEvalOp_def] \\ REPEAT STRIP_TAC
+  \\ REPEAT BasicProvers.CASE_TAC \\ fs []
+  \\ Cases_on `iEvalOpAux op a s1` \\ fs []
+  \\ Cases_on `x` \\ fs [] THEN1
+   (Cases_on `bEvalOp op a (bvi_to_bvl s1)` \\ fs []
+    \\ Cases_on `x` \\ fs [] \\ SRW_TAC [] [bvl_to_bvi_def])
+  \\ Cases_on `x'` \\ Cases_on `op` \\ fs [iEvalOpAux_def]
+  \\ Cases_on `a` \\ fs []);
 
 val domain_spt_set = prove(
   ``!t. domain (spt_set f t) = domain t``,
-  Induct \\ fs [spt_set_def,domain_def]);
+  Induct \\ fs [spt_set_def,sptreeTheory.domain_def]);
 
-val bEvalOp_bvp_to_bvl = prove(
-  ``(bEvalOp op a s1 = SOME (x0,s2)) /\ state_rel s1 t1 ==>
-    (bEvalOp op a (bvp_to_bvl t1) = SOME (x0,s2 with code := spt_set ARB t1.code))``,
-  fs [bvp_to_bvl_def,state_rel_def]
-  \\ Cases_on `op` \\ fs [bEvalOp_def]
-  \\ REPEAT BasicProvers.CASE_TAC \\ fs []
-  \\ CCONTR_TAC \\ fs [LET_DEF] \\ SRW_TAC [] []
-  \\ fs [bvl_state_explode] \\ fs []
-  \\ POP_ASSUM MP_TAC \\ fs [domain_spt_set]
-  \\ fs [code_rel_def]);
+val spt_set_LN = prove(
+  ``!t. spt_set f t = LN <=> t = LN``,
+  Cases \\ EVAL_TAC);
+
+val wf_spt_set = prove(
+  ``!t f. wf (spt_set f t) = wf t``,
+  Induct \\ fs [wf_def,spt_set_def,spt_set_LN]);
+
+val spt_set_spt_set = prove(
+  ``!t. spt_set (K ARB) (spt_set (K ARB) t) = spt_set (K ARB) t``,
+  Induct \\ fs [spt_set_def]);
+
+val lemmas = prove(
+  ``(2 + 2 * n - 1 = 2 * n + 1:num) /\
+    (2 + 2 * n' = 2 * n'' + 2 <=> n' = n'':num) /\
+    (2 * m = 2 * n <=> (m = n)) /\
+    ((2 * n'' + 1) DIV 2 = n'') /\
+    ((2 * n) DIV 2 = n) /\
+    (2 + 2 * n' <> 2 * n'' + 1) /\
+    (2 * m + 1 <> 2 * n' + 2)``,
+  REPEAT STRIP_TAC \\ SIMP_TAC std_ss []
+  THEN1 DECIDE_TAC
+  THEN1 DECIDE_TAC
+  THEN1 DECIDE_TAC
+  \\ fs [ONCE_REWRITE_RULE [MULT_COMM] MULT_DIV]
+  \\ fs [ONCE_REWRITE_RULE [MULT_COMM] DIV_MULT]
+  \\ IMP_RES_TAC (METIS_PROVE [] ``(m = n) ==> (m MOD 2 = n MOD 2)``)
+  \\ POP_ASSUM MP_TAC \\ SIMP_TAC std_ss []
+  \\ ONCE_REWRITE_TAC [MATCH_MP (GSYM MOD_PLUS) (DECIDE ``0 < 2:num``)]
+  \\ EVAL_TAC \\ fs [MOD_EQ_0,ONCE_REWRITE_RULE [MULT_COMM] MOD_EQ_0]);
+
+val IN_domain = store_thm("IN_domain",
+  ``!n x t1 t2.
+      (n IN domain LN <=> F) /\
+      (n IN domain (LS x) <=> (n = 0)) /\
+      (n IN domain (BN t1 t2) <=>
+         n <> 0 /\ (if EVEN n then ((n-1) DIV 2) IN domain t1
+                              else ((n-1) DIV 2) IN domain t2)) /\
+      (n IN domain (BS t1 x t2) <=>
+         n = 0 \/ (if EVEN n then ((n-1) DIV 2) IN domain t1
+                             else ((n-1) DIV 2) IN domain t2))``,
+  fs [domain_def] \\ REPEAT STRIP_TAC
+  \\ Cases_on `n = 0` \\ fs []
+  \\ Cases_on `EVEN n` \\ fs []
+  \\ fs [GSYM ODD_EVEN]
+  \\ IMP_RES_TAC EVEN_ODD_EXISTS
+  \\ fs [ADD1] \\ fs [lemmas]
+  \\ Cases_on `m` \\ fs [MULT_CLAUSES]
+  \\ REPEAT STRIP_TAC \\ EQ_TAC \\ REPEAT STRIP_TAC
+  \\ fs [lemmas])
+
+val lookup_spt_set_K = prove(
+  ``!t n. lookup n (spt_set (K x) t) = if n IN domain t then SOME x else NONE``,
+  Induct \\ fs [IN_domain,spt_set_def,lookup_def]
+  \\ REPEAT STRIP_TAC \\ Cases_on `n = 0` \\ fs []
+  \\ Cases_on `EVEN n` \\ fs []);
+
+val iEvalOp_bvp_to_bvi = prove(
+  ``(iEvalOp op a s1 = SOME (x0,s2)) /\ state_rel s1 t1 ==>
+    (iEvalOp op a (bvp_to_bvi t1) =
+      SOME (x0,s2 with code := spt_set (K ARB) t1.code))``,
+  fs [state_rel_def]
+  \\ ONCE_REWRITE_TAC [EQ_SYM_EQ] \\ fs []
+  \\ fs [iEvalOp_def] \\ REPEAT STRIP_TAC
+  \\ Cases_on `iEvalOpAux op a s1` \\ fs []
+  \\ REVERSE (Cases_on `x`) \\ fs [] THEN1
+   (Cases_on `op` \\ fs [iEvalOpAux_def]
+    \\ SRW_TAC [] [] \\ fs [] \\ SRW_TAC [] []
+    \\ fs [bvp_to_bvi_def,bvi_state_explode]
+    \\ Cases_on `a` \\ fs []
+    \\ SRW_TAC [] [] \\ fs [] \\ SRW_TAC [] []
+    \\ fs [bvp_to_bvi_def,bvi_state_explode])
+  \\ `iEvalOpAux op a (bvp_to_bvi t1) = SOME NONE` by
+   (Cases_on `op` \\ fs [iEvalOpAux_def]
+    \\ REPEAT BasicProvers.CASE_TAC \\ fs [])
+  \\ `bvi_to_bvl (bvp_to_bvi t1) = bvi_to_bvl s1` by ALL_TAC THEN1
+   (fs [bvi_to_bvl_def,bvp_to_bvi_def,code_rel_def,wf_spt_set,
+        spt_eq_thm,spt_set_spt_set,lookup_spt_set_K]) \\ fs []
+  \\ Cases_on `bEvalOp op a (bvi_to_bvl s1)` \\ fs []
+  \\ Cases_on `x` \\ fs []
+  \\ fs [bvl_to_bvi_def,bvp_to_bvi_def]);
 
 val lookup_list_to_num_set = prove(
   ``!xs. lookup x (list_to_num_set xs) = if MEM x xs then SOME () else NONE``,
@@ -296,15 +375,15 @@ val consume_space_add_space = prove(
     SOME (t with locals := env1)``,
   fs [consume_space_def,add_space_def,bvp_state_explode] \\ DECIDE_TAC);
 
-val bComp_correct = prove(
+val iComp_correct = prove(
   ``!xs env s1 res s2 t1 n corr tail live.
-      (bEval (xs,env,s1) = (res,s2)) /\ res <> Error /\
+      (iEval (xs,env,s1) = (res,s2)) /\ res <> Error /\
       var_corr env corr t1 /\ (LENGTH xs <> 1 ==> ~tail) /\
       (!k. n <= k ==> (lookup k t1.locals = NONE)) /\
       state_rel s1 t1 /\ EVERY (\n. lookup n t1.locals <> NONE) live /\
       (isException res ==> jump_exc t1 <> NONE) ==>
       ?t2 prog pres vs next_var.
-        (bComp n corr tail live xs = (prog,vs,next_var)) /\
+        (iComp n corr tail live xs = (prog,vs,next_var)) /\
         (pEval (prog,t1) = (pres,t2)) /\ state_rel s2 t2 /\
         (case pres of
          | SOME r =>
@@ -330,36 +409,36 @@ val bComp_correct = prove(
                    | Result xs => var_corr xs vs t2
                    | _ => F)``,
   SIMP_TAC std_ss [Once EQ_SYM_EQ]
-  \\ recInduct bEval_ind \\ REPEAT STRIP_TAC
-  \\ FULL_SIMP_TAC std_ss [bComp_def,pEval_def,bEval_def]
+  \\ recInduct iEval_ind \\ REPEAT STRIP_TAC
+  \\ FULL_SIMP_TAC std_ss [iComp_def,pEval_def,iEval_def]
   THEN1 (* NIL *)
     (SRW_TAC [] [var_corr_def]
      \\ CCONTR_TAC \\ FULL_SIMP_TAC std_ss [NOT_LESS]
      \\ RES_TAC \\ FULL_SIMP_TAC std_ss [])
   THEN1 (* CONS *)
-   (`?c1 v1 n1. bComp n corr F live [x] = (c1,v1,n1)` by METIS_TAC [PAIR]
-    \\ `?c2 vs n2. bComp n1 corr F (HD v1::live) (y::xs) = (c2,vs,n2)` by
+   (`?c1 v1 n1. iComp n corr F live [x] = (c1,v1,n1)` by METIS_TAC [PAIR]
+    \\ `?c2 vs n2. iComp n1 corr F (HD v1::live) (y::xs) = (c2,vs,n2)` by
           METIS_TAC [PAIR]
     \\ FULL_SIMP_TAC std_ss [LET_DEF,pEval_def]
-    \\ Cases_on `bEval ([x],env,s)`
+    \\ Cases_on `iEval ([x],env,s)`
     \\ Cases_on `q` \\ FULL_SIMP_TAC (srw_ss()) [isException_def]
     \\ FIRST_X_ASSUM (MP_TAC o Q.SPECL [`t1`,`n`,`corr`,`F`,`live`])
     \\ FULL_SIMP_TAC std_ss [isException_def] \\ REPEAT STRIP_TAC
     \\ Cases_on `pres` \\ FULL_SIMP_TAC std_ss [isResult_def]
-    \\ Cases_on `bEval (y::xs,env,r)`
+    \\ Cases_on `iEval (y::xs,env,r)`
     \\ Cases_on `q` \\ FULL_SIMP_TAC (srw_ss()) [isResult_def,isException_def]
     \\ FIRST_X_ASSUM (MP_TAC o Q.SPECL [`t2`,`n1`,`corr`,`F`,`HD v1::live`])
     \\ Q.PAT_ASSUM `isException res ==> bbb` MP_TAC
     \\ `EVERY (\n. lookup n t2.locals <> NONE) (HD v1::live)` by
-     (IMP_RES_TAC bEval_SING_IMP \\ FULL_SIMP_TAC (srw_ss()) []
-      \\ IMP_RES_TAC bComp_SING_IMP \\ fs [var_corr_def,get_var_def]
+     (IMP_RES_TAC iEval_SING_IMP \\ FULL_SIMP_TAC (srw_ss()) []
+      \\ IMP_RES_TAC iComp_SING_IMP \\ fs [var_corr_def,get_var_def]
       \\ fs [EVERY_MEM] \\ REPEAT STRIP_TAC \\ RES_TAC
       \\ Cases_on `lookup n' t1.locals` \\ fs [] \\ METIS_TAC [])
     \\ FULL_SIMP_TAC std_ss [isException_def] \\ REPEAT STRIP_TAC
     \\ FULL_SIMP_TAC std_ss [] \\ SRW_TAC [] []
     \\ Cases_on `pres` \\ FULL_SIMP_TAC (srw_ss()) [var_corr_def]
-    \\ IMP_RES_TAC bEval_SING_IMP \\ FULL_SIMP_TAC (srw_ss()) []
-    \\ IMP_RES_TAC bComp_SING_IMP \\ FULL_SIMP_TAC (srw_ss()) []
+    \\ IMP_RES_TAC iEval_SING_IMP \\ FULL_SIMP_TAC (srw_ss()) []
+    \\ IMP_RES_TAC iComp_SING_IMP \\ FULL_SIMP_TAC (srw_ss()) []
     \\ REPEAT STRIP_TAC THEN1 DECIDE_TAC THEN1 DECIDE_TAC
     \\ FULL_SIMP_TAC std_ss [EVERY_MEM]
     THEN1 (REPEAT STRIP_TAC \\ RES_TAC \\ DECIDE_TAC)
@@ -389,28 +468,28 @@ val bComp_correct = prove(
     \\ FIRST_X_ASSUM (MP_TAC o Q.SPEC `k'`)
     \\ REPEAT STRIP_TAC \\ fs [jump_exc_NONE])
   THEN1 (* If *)
-   (`?c1 v1 n1. bComp n corr F live [x1] = (c1,v1,n1)` by METIS_TAC [PAIR]
-    \\ `?c2 v2 n2. bComp n1 corr tail live [x2] = (c2,v2,n2)` by METIS_TAC [PAIR]
-    \\ `?c3 v3 n3. bComp n2 corr tail live [x3] = (c3,v3,n3)` by METIS_TAC [PAIR]
+   (`?c1 v1 n1. iComp n corr F live [x1] = (c1,v1,n1)` by METIS_TAC [PAIR]
+    \\ `?c2 v2 n2. iComp n1 corr tail live [x2] = (c2,v2,n2)` by METIS_TAC [PAIR]
+    \\ `?c3 v3 n3. iComp n2 corr tail live [x3] = (c3,v3,n3)` by METIS_TAC [PAIR]
     \\ FULL_SIMP_TAC std_ss [LET_DEF,pEval_def]
     \\ Cases_on `tail` \\ FULL_SIMP_TAC std_ss [] THEN1
      (SIMP_TAC std_ss [pEval_def]
-      \\ Cases_on `bEval ([x1],env,s)` \\ FULL_SIMP_TAC (srw_ss()) []
+      \\ Cases_on `iEval ([x1],env,s)` \\ FULL_SIMP_TAC (srw_ss()) []
       \\ Cases_on `q` \\ FULL_SIMP_TAC (srw_ss()) []
       \\ FIRST_X_ASSUM (MP_TAC o Q.SPECL [`t1`,`n`,`corr`,`F`,`live`])
       \\ FULL_SIMP_TAC std_ss [] \\ STRIP_TAC
       \\ FULL_SIMP_TAC (srw_ss()) [isResult_def,isException_def]
       \\ Cases_on `pres`
       \\ FULL_SIMP_TAC (srw_ss()) [isResult_def,isException_def]
-      \\ IMP_RES_TAC bEval_SING_IMP \\ FULL_SIMP_TAC (srw_ss()) []
-      \\ IMP_RES_TAC bComp_SING_IMP \\ FULL_SIMP_TAC (srw_ss()) []
+      \\ IMP_RES_TAC iEval_SING_IMP \\ FULL_SIMP_TAC (srw_ss()) []
+      \\ IMP_RES_TAC iComp_SING_IMP \\ FULL_SIMP_TAC (srw_ss()) []
       \\ SRW_TAC [] []
       \\ Q.MATCH_ASSUM_RENAME_TAC `var_corr [w] [n5] t2` []
       \\ `get_var n5 t2 = SOME w` by FULL_SIMP_TAC (srw_ss()) [var_corr_def]
       \\ FULL_SIMP_TAC std_ss []
       \\ FULL_SIMP_TAC std_ss [LET_DEF]
       \\ CONV_TAC (DEPTH_CONV (DEPTH_CONV PairRules.PBETA_CONV))
-      \\ IMP_RES_TAC bComp_LESS_EQ
+      \\ IMP_RES_TAC iComp_LESS_EQ
       \\ `EVERY (\n. lookup n t2.locals <> NONE) live` by
         (fs [EVERY_MEM] \\ REPEAT STRIP_TAC \\ RES_TAC
          \\ Cases_on `lookup n' t1.locals` \\ fs [] \\ METIS_TAC [])
@@ -430,22 +509,22 @@ val bComp_correct = prove(
         THEN1 (REPEAT STRIP_TAC \\ FIRST_X_ASSUM MATCH_MP_TAC \\ DECIDE_TAC)
         \\ FULL_SIMP_TAC std_ss []))
     \\ SIMP_TAC std_ss [pEval_def]
-    \\ Cases_on `bEval ([x1],env,s)` \\ FULL_SIMP_TAC (srw_ss()) []
+    \\ Cases_on `iEval ([x1],env,s)` \\ FULL_SIMP_TAC (srw_ss()) []
     \\ Cases_on `q` \\ FULL_SIMP_TAC (srw_ss()) []
     \\ FIRST_X_ASSUM (MP_TAC o Q.SPECL [`t1`,`n`,`corr`,`F`,`live`])
     \\ FULL_SIMP_TAC std_ss [] \\ STRIP_TAC
     \\ FULL_SIMP_TAC (srw_ss()) [isResult_def,isException_def]
     \\ Cases_on `pres`
     \\ FULL_SIMP_TAC (srw_ss()) [isResult_def,isException_def]
-    \\ IMP_RES_TAC bEval_SING_IMP \\ FULL_SIMP_TAC (srw_ss()) []
-    \\ IMP_RES_TAC bComp_SING_IMP \\ FULL_SIMP_TAC (srw_ss()) []
+    \\ IMP_RES_TAC iEval_SING_IMP \\ FULL_SIMP_TAC (srw_ss()) []
+    \\ IMP_RES_TAC iComp_SING_IMP \\ FULL_SIMP_TAC (srw_ss()) []
     \\ SRW_TAC [] []
     \\ Q.MATCH_ASSUM_RENAME_TAC `var_corr [w] [n5] t2` []
     \\ `get_var n5 t2 = SOME w` by FULL_SIMP_TAC (srw_ss()) [var_corr_def]
     \\ FULL_SIMP_TAC std_ss []
     \\ FULL_SIMP_TAC std_ss [LET_DEF]
     \\ CONV_TAC (DEPTH_CONV (DEPTH_CONV PairRules.PBETA_CONV))
-    \\ IMP_RES_TAC bComp_LESS_EQ
+    \\ IMP_RES_TAC iComp_LESS_EQ
     \\ `EVERY (\n. lookup n t2.locals <> NONE) live` by
       (fs [EVERY_MEM] \\ REPEAT STRIP_TAC \\ RES_TAC
        \\ Cases_on `lookup n' t1.locals` \\ fs [] \\ METIS_TAC [])
@@ -458,7 +537,7 @@ val bComp_correct = prove(
       \\ FULL_SIMP_TAC std_ss []
       \\ Cases_on `pres` \\ FULL_SIMP_TAC (srw_ss()) []
       \\ Cases_on `res` \\ FULL_SIMP_TAC (srw_ss()) []
-      \\ IMP_RES_TAC bEval_SING_IMP \\ FULL_SIMP_TAC (srw_ss()) []
+      \\ IMP_RES_TAC iEval_SING_IMP \\ FULL_SIMP_TAC (srw_ss()) []
       \\ SRW_TAC [] []
       \\ Q.MATCH_ASSUM_RENAME_TAC `var_corr [w7] [n7] t7` []
       \\ `get_var n7 t7 = SOME w7` by FULL_SIMP_TAC (srw_ss()) [var_corr_def]
@@ -494,7 +573,7 @@ val bComp_correct = prove(
       \\ STRIP_TAC \\ FULL_SIMP_TAC std_ss []
       \\ Cases_on `pres` \\ FULL_SIMP_TAC (srw_ss()) []
       \\ Cases_on `res` \\ FULL_SIMP_TAC (srw_ss()) []
-      \\ IMP_RES_TAC bEval_SING_IMP \\ FULL_SIMP_TAC (srw_ss()) []
+      \\ IMP_RES_TAC iEval_SING_IMP \\ FULL_SIMP_TAC (srw_ss()) []
       \\ SRW_TAC [] []
       \\ Q.MATCH_ASSUM_RENAME_TAC `var_corr [w7] [n7] t7` []
       \\ `get_var n7 t7 = SOME w7` by FULL_SIMP_TAC (srw_ss()) [var_corr_def]
@@ -520,11 +599,11 @@ val bComp_correct = prove(
              \\ RES_TAC \\ FULL_SIMP_TAC std_ss [])
       \\ FULL_SIMP_TAC std_ss [jump_exc_NONE]))
   THEN1 (* Let *)
-   (`?c1 vs n1. bComp n corr F live xs = (c1,vs,n1)` by METIS_TAC [PAIR]
-    \\ `?c2 v2 n2. bComp n1 (vs ++ corr) tail live [x2] =
+   (`?c1 vs n1. iComp n corr F live xs = (c1,vs,n1)` by METIS_TAC [PAIR]
+    \\ `?c2 v2 n2. iComp n1 (vs ++ corr) tail live [x2] =
                    (c2,v2,n2)` by METIS_TAC [PAIR]
     \\ FULL_SIMP_TAC std_ss [LET_DEF,pEval_def]
-    \\ Cases_on `bEval (xs,env,s)`
+    \\ Cases_on `iEval (xs,env,s)`
     \\ REVERSE (Cases_on `q`) \\ FULL_SIMP_TAC (srw_ss()) []
     \\ FIRST_X_ASSUM (MP_TAC o Q.SPECL [`t1`,`n`,`corr`,`F`,`live`])
     \\ FULL_SIMP_TAC std_ss [] \\ STRIP_TAC
@@ -553,28 +632,27 @@ val bComp_correct = prove(
     \\ IMP_RES_TAC LIST_REL_LENGTH
     \\ FULL_SIMP_TAC (srw_ss()) [])
   THEN1 (* Raise *)
-   (`?c1 v1 n1. bComp n corr F live [x1] = (c1,v1,n1)` by METIS_TAC [PAIR]
+   (`?c1 v1 n1. iComp n corr F live [x1] = (c1,v1,n1)` by METIS_TAC [PAIR]
     \\ FULL_SIMP_TAC std_ss [LET_DEF,pEval_def,call_env_def]
-    \\ Cases_on `bEval ([x1],env,s)` \\ FULL_SIMP_TAC (srw_ss()) []
+    \\ Cases_on `iEval ([x1],env,s)` \\ FULL_SIMP_TAC (srw_ss()) []
     \\ Cases_on `q` \\ FULL_SIMP_TAC (srw_ss()) []
     \\ FIRST_X_ASSUM (MP_TAC o Q.SPECL [`t1`,`n`,`corr`,`F`,`live`])
     \\ FULL_SIMP_TAC std_ss [isException_def] \\ STRIP_TAC
     \\ FULL_SIMP_TAC (srw_ss()) [isResult_def,isException_def]
     \\ Cases_on `pres`
     \\ FULL_SIMP_TAC (srw_ss()) [isResult_def,isException_def]
-    \\ IMP_RES_TAC bEval_SING_IMP \\ FULL_SIMP_TAC (srw_ss()) []
-    \\ IMP_RES_TAC bComp_SING_IMP \\ FULL_SIMP_TAC (srw_ss()) []
+    \\ IMP_RES_TAC iEval_SING_IMP \\ FULL_SIMP_TAC (srw_ss()) []
+    \\ IMP_RES_TAC iComp_SING_IMP \\ FULL_SIMP_TAC (srw_ss()) []
     \\ SRW_TAC [] []
     \\ `get_var t t2 = SOME w` by fs [var_corr_def]
     \\ fs [] \\ Cases_on `jump_exc t2` \\ fs [res_list_def]
     \\ FULL_SIMP_TAC std_ss [state_rel_def]
     \\ IMP_RES_TAC jump_exc_IMP \\ fs []
     \\ fs [jump_exc_def])
-  THEN1 (* Handle *) cheat
   THEN1 (* Op *)
-   (`?c1 vs n1. bComp n corr F live xs = (c1,vs,n1)` by METIS_TAC [PAIR]
+   (`?c1 vs n1. iComp n corr F live xs = (c1,vs,n1)` by METIS_TAC [PAIR]
     \\ FULL_SIMP_TAC std_ss [LET_DEF,pEval_def]
-    \\ Cases_on `bEval (xs,env,s)`
+    \\ Cases_on `iEval (xs,env,s)`
     \\ REVERSE (Cases_on `q`) \\ FULL_SIMP_TAC (srw_ss()) []
     \\ FIRST_X_ASSUM (MP_TAC o Q.SPECL [`t1`,`n`,`corr`,`F`,`live`])
     \\ FULL_SIMP_TAC std_ss [] \\ STRIP_TAC
@@ -582,7 +660,7 @@ val bComp_correct = prove(
     \\ Cases_on `pres`
     \\ FULL_SIMP_TAC (srw_ss()) [isResult_def,isException_def]
     THEN1 SRW_TAC [] [pEval_def] THEN1 SRW_TAC [] [pEval_def]
-    \\ Cases_on `bEvalOp op a r` \\ fs []
+    \\ Cases_on `iEvalOp op a r` \\ fs []
     \\ PairCases_on `x` \\ fs [] \\ REV_FULL_SIMP_TAC std_ss []
     \\ (fn (hs,goal) => (REVERSE (`let tail = F in ^goal` by ALL_TAC))
            (hs,goal)) THEN1
@@ -609,15 +687,15 @@ val bComp_correct = prove(
     \\ IMP_RES_TAC get_vars_thm
     \\ `state_rel r (t2 with <|locals := env1; space := 0|>)` by
           (fs [state_rel_def] \\ NO_TAC)
-    \\ fs [LET_DEF,pEval_def,bAssign_def]
+    \\ fs [LET_DEF,pEval_def,iAssign_def]
     \\ Cases_on `op_space_reset op`
     \\ fs [pEval_def,cut_state_opt_def,cut_state_def,cut_env_def]
     \\ fs [pEvalOp_def,pEvalOpSpace_def]
-    \\ IMP_RES_TAC bEvalOp_bvp_to_bvl \\ fs []
+    \\ IMP_RES_TAC iEvalOp_bvp_to_bvi \\ fs []
     \\ fs [get_var_def,set_var_def,res_list_def,isResult_def]
-    \\ fs [call_env_def,bvl_to_bvp_def,isException_def]
-    \\ fs [state_rel_def] \\ IMP_RES_TAC bEvalOp_code \\ fs []
-    \\ IMP_RES_TAC bComp_LESS_EQ \\ fs [lookup_insert]
+    \\ fs [call_env_def,bvi_to_bvp_def,isException_def]
+    \\ fs [state_rel_def] \\ IMP_RES_TAC iEvalOp_code \\ fs []
+    \\ IMP_RES_TAC iComp_LESS_EQ \\ fs [lookup_insert]
     THEN1
      (REPEAT STRIP_TAC THEN1 DECIDE_TAC
       THEN1 (SRW_TAC [] [] THEN1 DECIDE_TAC
@@ -647,11 +725,11 @@ val bComp_correct = prove(
     \\ Cases_on `op_space_req op = 0` \\ fs [pEval_def]
     \\ fs [pEval_def,cut_state_opt_def,cut_state_def,cut_env_def]
     \\ fs [pEvalOp_def,pEvalOpSpace_def,LET_DEF]
-    \\ IMP_RES_TAC bEvalOp_bvp_to_bvl \\ fs []
+    \\ IMP_RES_TAC iEvalOp_bvp_to_bvi \\ fs []
     \\ fs [get_var_def,set_var_def,res_list_def,isResult_def]
-    \\ fs [call_env_def,bvl_to_bvp_def,isException_def]
-    \\ fs [state_rel_def] \\ IMP_RES_TAC bEvalOp_code \\ fs []
-    \\ IMP_RES_TAC bComp_LESS_EQ \\ fs [lookup_insert]
+    \\ fs [call_env_def,bvi_to_bvp_def,isException_def]
+    \\ fs [state_rel_def] \\ IMP_RES_TAC iEvalOp_code \\ fs []
+    \\ IMP_RES_TAC iComp_LESS_EQ \\ fs [lookup_insert]
     THEN1
      (REPEAT STRIP_TAC THEN1 DECIDE_TAC
       THEN1 (SRW_TAC [] [] THEN1 DECIDE_TAC
@@ -706,7 +784,7 @@ val bComp_correct = prove(
          \\ POP_ASSUM MP_TAC \\ POP_ASSUM MP_TAC \\ fs [jump_exc_def])
       \\ fs [var_corr_def,get_var_def]))
   THEN1 (* Tick *)
-   (`?c1 v1 n1. bComp n corr tail live [x] = (c1,v1,n1)` by METIS_TAC [PAIR]
+   (`?c1 v1 n1. iComp n corr tail live [x] = (c1,v1,n1)` by METIS_TAC [PAIR]
     \\ FULL_SIMP_TAC std_ss [LET_DEF,pEval_def]
     \\ Cases_on `t1.clock = 0` \\ FULL_SIMP_TAC std_ss []
     THEN1 (fs [state_rel_def,res_list_def,
@@ -719,12 +797,13 @@ val bComp_correct = prove(
     \\ FIRST_X_ASSUM (MP_TAC o Q.SPECL [`dec_clock t1`,`n`,`corr`,`tail`,`live`])
     \\ FULL_SIMP_TAC std_ss []
     \\ MATCH_MP_TAC IMP_IMP \\ STRIP_TAC
-    \\ FULL_SIMP_TAC (srw_ss()) [var_corr_def,dec_clock_def,
-         get_var_def,state_rel_def,bvlTheory.dec_clock_def,jump_exc_NONE])
+    \\ FULL_SIMP_TAC (srw_ss()) [var_corr_def,bvpTheory.dec_clock_def,
+         get_var_def,state_rel_def,bviTheory.dec_clock_def,jump_exc_NONE])
   THEN1 (* Call *)
-   (`?c1 vs n1. bComp n corr F live xs = (c1,vs,n1)` by METIS_TAC [PAIR]
+   (REVERSE (Cases_on `handler`) THEN1 cheat \\ fs []
+    \\ `?c1 vs n1. iComp n corr F live xs = (c1,vs,n1)` by METIS_TAC [PAIR]
     \\ FULL_SIMP_TAC std_ss [LET_DEF,pEval_def,call_env_def]
-    \\ Cases_on `bEval (xs,env,s1)`
+    \\ Cases_on `iEval (xs,env,s1)`
     \\ REVERSE (Cases_on `q`) \\ FULL_SIMP_TAC (srw_ss()) []
     \\ FIRST_X_ASSUM (MP_TAC o Q.SPECL [`t1`,`n`,`corr`,`F`,`live`])
     \\ FULL_SIMP_TAC std_ss [] \\ STRIP_TAC
@@ -743,18 +822,21 @@ val bComp_correct = prove(
     \\ FULL_SIMP_TAC std_ss []
     \\ IMP_RES_TAC find_code_lemma
     \\ FULL_SIMP_TAC (srw_ss()) [] \\ POP_ASSUM (K ALL_TAC)
-    \\ FULL_SIMP_TAC std_ss [bCompile_def,isException_def]
+    \\ FULL_SIMP_TAC std_ss [iCompile_def,isException_def]
     \\ Q.PAT_ASSUM `(res,s2) = bb` (ASSUME_TAC o GSYM)
     \\ FULL_SIMP_TAC std_ss []
     \\ Cases_on `tail` THEN1
-     (FIRST_X_ASSUM (MP_TAC o Q.SPECL [`call_env args (dec_clock t2)`,
+     (`iEval ([exp],args,dec_clock r) = (res,s2)` by ALL_TAC THEN1
+        (Cases_on `iEval ([exp],args,dec_clock r)` \\ fs []
+         \\ Cases_on `q` \\ fs []) \\ fs []
+      \\ FIRST_X_ASSUM (MP_TAC o Q.SPECL [`call_env args (dec_clock t2)`,
            `LENGTH (args:bc_value list)`,
            `GENLIST I (LENGTH (args:bc_value list))`,`T`,`[]`])
       \\ FULL_SIMP_TAC std_ss []
       \\ MATCH_MP_TAC IMP_IMP \\ STRIP_TAC THEN1
-       (FULL_SIMP_TAC (srw_ss()) [state_rel_def,dec_clock_def,call_env_def,
-          bvlTheory.dec_clock_def,var_corr_def,get_var_def,LIST_REL_REVERSE,
-          LIST_REL_lookup_fromList,lookup_fromList_NONE,jump_exc_NONE])
+       (FULL_SIMP_TAC (srw_ss()) [state_rel_def,bvpTheory.dec_clock_def,
+          bviTheory.dec_clock_def,var_corr_def,get_var_def,LIST_REL_REVERSE,
+          LIST_REL_lookup_fromList,lookup_fromList_NONE,jump_exc_NONE,call_env_def])
       \\ STRIP_TAC \\ fs [LET_DEF]
       \\ MP_TAC (Q.SPECL [`prog`,
             `call_env args (dec_clock t2)`] pEval_pOptimise) \\ fs []
@@ -765,7 +847,8 @@ val bComp_correct = prove(
       \\ REPEAT STRIP_TAC \\ fs []
       \\ Cases_on `pres` \\ fs [] \\ FULL_SIMP_TAC std_ss []
       \\ REPEAT STRIP_TAC \\ FULL_SIMP_TAC std_ss []
-      \\ FULL_SIMP_TAC (srw_ss()) [call_env_def,dec_clock_def]
+      \\ FULL_SIMP_TAC (srw_ss()) [call_env_def,
+           bviTheory.dec_clock_def,bvpTheory.dec_clock_def]
       \\ REV_FULL_SIMP_TAC (srw_ss()) [])
     \\ `domain (list_to_num_set (live ++ corr)) SUBSET domain t2.locals` by
      (fs [SUBSET_DEF,domain_lookup,lookup_list_to_num_set,EVERY_MEM]
@@ -775,16 +858,19 @@ val bComp_correct = prove(
       \\ fs [var_corr_def,get_var_def]
       \\ IMP_RES_TAC MEM_LIST_REL \\ fs [])
     \\ fs [cut_env_def]
-    \\ Q.ABBREV_TAC `env2 = mk_wf (inter t2.locals (list_to_num_set (live ++ corr)))`
+    \\ `iEval ([exp],args,dec_clock r) = (res,s2)` by ALL_TAC THEN1
+     (Cases_on `iEval ([exp],args,dec_clock r)` \\ fs []
+      \\ Cases_on `q` \\ fs []) \\ fs []
+    \\ Q.ABBREV_TAC `env2 = (inter t2.locals (list_to_num_set (live ++ corr)))`
     \\ FIRST_X_ASSUM (MP_TAC o Q.SPECL
           [`call_env args (push_env env2 F (dec_clock t2))`,
            `LENGTH (args:bc_value list)`,
            `GENLIST I (LENGTH (args:bc_value list))`,`T`,`[]`])
     \\ FULL_SIMP_TAC std_ss []
     \\ MATCH_MP_TAC IMP_IMP \\ STRIP_TAC THEN1
-       (FULL_SIMP_TAC (srw_ss()) [state_rel_def,dec_clock_def,call_env_def,
-          bvlTheory.dec_clock_def,var_corr_def,get_var_def,LIST_REL_REVERSE,
-          LIST_REL_lookup_fromList,lookup_fromList_NONE,push_env_def]
+       (FULL_SIMP_TAC (srw_ss()) [state_rel_def,bvpTheory.dec_clock_def,
+          bviTheory.dec_clock_def,var_corr_def,get_var_def,LIST_REL_REVERSE,
+          LIST_REL_lookup_fromList,lookup_fromList_NONE,push_env_def,call_env_def]
         \\ STRIP_TAC \\ FULL_SIMP_TAC std_ss []
         \\ `jump_exc t2 <> NONE` by FULL_SIMP_TAC std_ss []
         \\ Cases_on `jump_exc t2` \\ fs []
@@ -806,7 +892,8 @@ val bComp_correct = prove(
     \\ FULL_SIMP_TAC std_ss [isResult_def,isException_def]
     THEN1
      (IMP_RES_TAC jump_exc_IMP
-      \\ FULL_SIMP_TAC (srw_ss()) [call_env_def,push_env_def,dec_clock_def]
+      \\ FULL_SIMP_TAC (srw_ss()) [call_env_def,push_env_def,
+           bvpTheory.dec_clock_def,bviTheory.dec_clock_def]
       \\ SIMP_TAC (srw_ss()) [jump_exc_def]
       \\ Cases_on `t2.handler = LENGTH t2.stack` THEN1
        (FULL_SIMP_TAC std_ss [Q.SPEC `x::xs` LAST_N_LENGTH
@@ -819,9 +906,9 @@ val bComp_correct = prove(
          <| stack := t2.stack; locals := env2 |>)` by ALL_TAC THEN1
      (Q.PAT_ASSUM `xx = t2'.stack` (ASSUME_TAC o GSYM)
       \\ FULL_SIMP_TAC (srw_ss()) [call_env_def,push_env_def,
-           pop_env_def,dec_clock_def])
+           pop_env_def,bvpTheory.dec_clock_def,bviTheory.dec_clock_def])
     \\ fs [set_var_def,state_rel_def]
-    \\ IMP_RES_TAC bComp_LESS_EQ
+    \\ IMP_RES_TAC iComp_LESS_EQ
     \\ REPEAT STRIP_TAC THEN1 DECIDE_TAC
     THEN1
      (UNABBREV_ALL_TAC
@@ -858,7 +945,8 @@ val bComp_correct = prove(
       \\ `k <> n1` by ALL_TAC \\ fs [] \\ CCONTR_TAC \\ fs []
       \\ RES_TAC \\ FULL_SIMP_TAC std_ss [])
     \\ REPEAT (FULL_SIMP_TAC (srw_ss()) [var_corr_def,get_var_def,lookup_insert,
-                call_env_def,push_env_def,dec_clock_def]
+                call_env_def,push_env_def,bvpTheory.dec_clock_def,
+                bviTheory.dec_clock_def]
                \\ FULL_SIMP_TAC (srw_ss()) [jump_exc_def]
                \\ REPEAT BasicProvers.FULL_CASE_TAC)));
 
@@ -866,18 +954,18 @@ val option_case_NONE = prove(
   ``(case pres of NONE => F | SOME x => p x) <=> ?r. (pres = SOME r) /\ p r``,
   Cases_on `pres` \\ SRW_TAC [] []);
 
-val bCompile_lemma = bComp_correct
+val iCompile_lemma = iComp_correct
   |> Q.SPECL [`[exp]`,`env`,`s1`,`res`,`s2`,`t1`,`n`,`GENLIST I n`,`T`,`[]`]
-  |> SIMP_RULE std_ss [LENGTH,GSYM bCompile_def,option_case_NONE,
+  |> SIMP_RULE std_ss [LENGTH,GSYM iCompile_def,option_case_NONE,
        PULL_EXISTS,EVERY_DEF];
 
-val bCompile_correct = store_thm("bCompile_correct",
-  ``^(bCompile_lemma |> concl |> dest_imp |> fst) ==>
+val iCompile_correct = store_thm("iCompile_correct",
+  ``^(iCompile_lemma |> concl |> dest_imp |> fst) ==>
     ?t2 prog vs next_var r.
-      pEval (bCompile n exp,t1) = (SOME r,t2) /\
+      pEval (iCompile n exp,t1) = (SOME r,t2) /\
       state_rel s2 t2 /\ res_list r = res``,
-  REPEAT STRIP_TAC \\ MP_TAC bCompile_lemma \\ fs []
-  \\ REPEAT STRIP_TAC \\ fs [bCompile_def,LET_DEF]
+  REPEAT STRIP_TAC \\ MP_TAC iCompile_lemma \\ fs []
+  \\ REPEAT STRIP_TAC \\ fs [iCompile_def,LET_DEF]
   \\ MP_TAC (Q.SPECL [`prog`,`t1`] pEval_pOptimise) \\ fs []
   \\ `r <> Error` by (REPEAT STRIP_TAC \\ fs [res_list_def]) \\ fs []);
 
